\subsection{$\rho_{[cpr\mapsto id]}(R_1 \Join R_2) = (\rho_{[cpr\mapsto id]} R_1) \Join R_2$}

\begin{table}[ht]
	\begin{tabular}{l}
		$\bm{R_{LHS}}$  \\
		$\rho_{[cpr\mapsto id]}(R_1 \Join R_2)$  \\
		$A(R_{LHS}) = \rho_{[cpr\mapsto id]}(A(R_1) \Join A(R_2))$  \\
		$A(R_{LHS}) = \{id, address\} \Join \{id, name\}$  \\
		$A(R_{LHS}) = \{id, address, name\}$
	\end{tabular}
\end{table}

\begin{table}[ht]
	\begin{tabular}{l}
		$\bm{R_{RHS}}$ \\
	 	$(\rho_{[cpr\mapsto id]} R_1) \Join R_2$ \\
		$A(R_{RHS}) = (\rho_{[cpr\mapsto id]}A(R_1)) \Join A(R_2)$ \\
		$A(R_{RHS}) = \{id, address\} \Join \{cpr, name\}$ \\
		$A(R_{RHS}) = \{id, address, cpr, name\}$
	\end{tabular}
\end{table}
\FloatBarrier

This equality is not true as the right-hand side relation $(R_{RHS})$ results to the cartesian product of $R_1$ and $R_2$, as there aren't any common attributes, due to the renaming of cpr to id in $R_1$.
For this equality to be true the $R_{RHS}$ should also have renamed the $R_2$ relations cpr to id,\\
$R_{RHS} = (\rho_{[cpr\mapsto id]} R_1) \Join (\rho_{[cpr\mapsto id]} R_2)$\\
as this isn't the case the equality is false.\\\\
