\subsection{$\pi_{id,name,address}(\sigma_{cpr=id}(\rho_{[cpr \mapsto id]}R_1 \times R_2)) = (\rho_{[cpr \mapsto id]}R_1) \Join (\rho_{[cpr \mapsto id]}R_2)$}

\begin{table}[ht]
	\begin{tabular}{l}
		 $\bm{R_{LHS}}$ \\
		 $\pi_{id,name,address}(\sigma_{cpr=id}(\rho_{[cpr \mapsto id]}R_1 \times R_2))$   \\
		 $A(R_{LHS}) = \pi_{id,name,address}(\sigma_{cpr=id}(\rho_{[cpr \mapsto id]}A(R_1) \times A(R_2)))$   \\
		 $A(R_{LHS}) = \pi_{id,name,address}(\sigma_{cpr=id}(\{id, address, cpr, name\} \times \{id, name\}))$  \\
		 $A(R_{LHS}) = \{id, address, name\}$ 
	\end{tabular}
\end{table}

\begin{table}[ht]
	\begin{tabular}{l}
		 $\bm{R_{RHS}}$ \\
		 $(\rho_{[cpr \mapsto id]}R_1) \Join (\rho_{[cpr \mapsto id]}R_2)$ \\
		 $A(R_{RHS}) = (\rho_{[cpr \mapsto id]}A(R_1) \Join (\rho_{[cpr \mapsto id]}A(R_2))$ \\
		 $A(R_{RHS}) = \{id, address\} \Join \{id, name\}$ \\
		 $A(R_{RHS}) = \{id, address, name\}$
	\end{tabular}
\end{table}
\FloatBarrier

This is true as both the left-hand side relation and the right-hand side relation have the same attributes and tuples.\\\\